src/Std/Tactic/BVDecide/Bitblast/BVExpr/Circuit/Lemmas/Expr.lean
@@ -32,28 +32,40 @@ open Std.Sat
 open Std.Sat.AIG
 
 namespace BVExpr
+
+namespace Cache
+
+abbrev Inv (assign : Assignment) (aig : AIG BVBit) (cache : Cache aig) : Prop :=
+  ∀ k (h1 : k ∈ cache.map), ∀ (i : Nat) (h2 : i < k.w),
+    ⟦aig, ⟨(cache.map.get k h1)[i].1, (cache.map.get k h1)[i].2, cache.hbound ..⟩, assign.toAIGAssignment⟧
+      =
+    (k.expr.eval assign).getLsbD i
+
+theorem Inv_empty (aig : AIG BVBit) : Inv assign aig Cache.empty := sorry
+
+theorem Inv_cast (cache : Cache aig1) (hle : aig1.decls.size ≤ aig2.decls.size)
+    (hinv : Inv assign aig1 cache):
+    Inv assign aig2 (cache.cast hle) := sorry
+
+theorem Inv_insert (cache : Cache aig) (expr : BVExpr w) (refs : AIG.RefVec aig w)
+    (hinv : Inv assign aig cache)
+    (hrefs : ∀ (idx : Nat) (hidx : idx < w), ⟦aig, refs.get idx hidx, assign.toAIGAssignment⟧ = (expr.eval assign).getLsbD idx) :
+    Inv assign aig (cache.insert expr refs) := sorry
+
+theorem denote_eq_eval_of_get?_eq_some_of_Inv (cache : Cache aig) (expr : BVExpr w)
+    (refs : AIG.RefVec aig w) (hsome : cache.get? expr = some refs) (hinv : Inv assign aig cache) :
+    ∀ (i : Nat) (h : i < w),
+      ⟦aig,  refs.get i h, assign.toAIGAssignment⟧ = (expr.eval assign).getLsbD i := sorry
+
+end Cache
+
 namespace bitblast
 
-/-
-theorem go_val_eq_bitblast (aig : AIG BVBit) (expr : BVExpr w) :
-    (go aig expr).val = bitblast aig expr := by
+theorem goCache_val_eq_bitblast (aig : AIG BVBit) (expr : BVExpr w) :
+    (goCache aig expr .empty).result.val = bitblast aig expr := by
   rfl
 
-theorem go_denote_mem_prefix (aig : AIG BVBit) (expr : BVExpr w) (assign : Assignment) (start : Nat)
-    (hstart) :
-    ⟦
-      (go aig expr).val.aig,
-      ⟨start, inv, by apply Nat.lt_of_lt_of_le; exact hstart; apply (go aig expr).property⟩,
-      assign.toAIGAssignment
-    ⟧
-      =
-    ⟦aig, ⟨start, inv, hstart⟩, assign.toAIGAssignment⟧ := by
-  apply denote.eq_of_isPrefix (entry := ⟨aig, start, inv, hstart⟩)
-  apply IsPrefix.of
-  · intros
-    apply go_decl_eq
-  · intros
-    apply (go aig expr).property
+/-
 
 theorem go_denote_eq (aig : AIG BVBit) (expr : BVExpr w) (assign : Assignment) :
     ∀ (idx : Nat) (hidx : idx < w),
@@ -62,10 +74,6 @@ theorem go_denote_eq (aig : AIG BVBit) (expr : BVExpr w) (assign : Assignment) :
         (expr.eval assign).getLsbD idx := by
   intro idx hidx
   induction expr generalizing aig idx with
-  | const =>
-    simp [go, denote_blastConst]
-  | var =>
-    simp [go, hidx, denote_blastVar]
   | append lhs rhs hw lih rih =>
     rename_i lw rw
     subst hw
@@ -122,90 +130,234 @@ theorem go_denote_eq (aig : AIG BVBit) (expr : BVExpr w) (assign : Assignment) :
       · simp [Ref.hgate]
     · intros
       rw [← rih]
-  | bin lhs op rhs lih rih =>
-    cases op with
-    | and =>
-      simp only [go, RefVec.denote_zip, denote_mkAndCached, rih, eval_bin, BVBinOp.eval_and,
-        BitVec.getLsbD_and]
-      simp only [go_val_eq_bitblast, RefVec.get_cast]
-      rw [AIG.LawfulVecOperator.denote_input_vec (f := bitblast)]
-      rw [← go_val_eq_bitblast]
-      rw [lih]
-    | or =>
-      simp only [go, RefVec.denote_zip, denote_mkOrCached, rih, eval_bin, BVBinOp.eval_or,
-        BitVec.getLsbD_or]
-      simp only [go_val_eq_bitblast, RefVec.get_cast]
-      rw [AIG.LawfulVecOperator.denote_input_vec (f := bitblast)]
-      rw [← go_val_eq_bitblast]
-      rw [lih]
-    | xor =>
-      simp only [go, RefVec.denote_zip, denote_mkXorCached, rih, eval_bin, BVBinOp.eval_xor,
-        BitVec.getLsbD_xor]
-      simp only [go_val_eq_bitblast, RefVec.get_cast]
-      rw [AIG.LawfulVecOperator.denote_input_vec (f := bitblast)]
-      rw [← go_val_eq_bitblast]
-      rw [lih]
-    | add =>
-      simp only [go, eval_bin, BVBinOp.eval_add]
-      apply denote_blastAdd
-      · intros
-        dsimp only
-        rw [go_denote_mem_prefix]
-        rw [← lih (aig := aig)]
-        · simp
-        · assumption
-        · simp [Ref.hgate]
-      · intros
-        rw [← rih]
-    | mul =>
-      simp only [go, eval_bin, BVBinOp.eval_mul]
-      apply denote_blastMul
-      · intros
-        dsimp only
-        rw [go_denote_mem_prefix]
-        rw [← lih (aig := aig)]
-        · simp
-        · assumption
-        · simp [Ref.hgate]
-      · intros
-        rw [← rih]
-    | udiv =>
-      simp only [go, eval_bin, BVBinOp.eval_udiv]
-      apply denote_blastUdiv
-      · intros
-        dsimp only
-        rw [go_denote_mem_prefix]
-        rw [← lih (aig := aig)]
-        · simp
-        · assumption
-        · simp [Ref.hgate]
-      · intros
-        rw [← rih]
-    | umod =>
-      simp only [go, eval_bin, BVBinOp.eval_umod]
-      apply denote_blastUmod
-      · intros
-        dsimp only
-        rw [go_denote_mem_prefix]
-        rw [← lih (aig := aig)]
-        · simp
-        · assumption
-        · simp [Ref.hgate]
-      · intros
-        rw [← rih]
-  | un op expr ih =>
-    cases op with
-    | not => simp [go, ih, hidx]
-    | rotateLeft => simp [go, ih, hidx, ← BitVec.getLsbD_eq_getElem]
-    | rotateRight => simp [go, ih, hidx, ← BitVec.getLsbD_eq_getElem]
-    | arithShiftRightConst n =>
-      rename_i w
-      have : ¬(w ≤ idx) := by omega
-      simp [go, ih, this, BitVec.getLsbD_sshiftRight, BitVec.msb_eq_getLsbD_last ]
 -/
-end bitblast
 
-axiom mySorry {α : Sort u} : α
+theorem go_denote_mem_prefix (aig : AIG BVBit) (expr : BVExpr w) (assign : Assignment)
+    (cache : Cache aig) (start : Nat) (hstart) :
+    ⟦
+      (go aig expr cache).result.val.aig,
+      ⟨start, inv, by apply Nat.lt_of_lt_of_le; exact hstart; apply (go aig expr cache).result.property⟩,
+      assign.toAIGAssignment
+    ⟧
+      =
+    ⟦aig, ⟨start, inv, hstart⟩, assign.toAIGAssignment⟧ := by
+  apply denote.eq_of_isPrefix (entry := ⟨aig, start, inv, hstart⟩)
+  apply IsPrefix.of
+  · intros
+    apply go_decl_eq
+  · intros
+    apply (go aig expr cache).result.property
+
+theorem goCache_denote_mem_prefix (aig : AIG BVBit) (expr : BVExpr w) (assign : Assignment)
+    (cache : Cache aig) (start : Nat) (hstart) :
+    ⟦
+      (goCache aig expr cache).result.val.aig,
+      ⟨start, inv, by apply Nat.lt_of_lt_of_le; exact hstart; apply (goCache aig expr cache).result.property⟩,
+      assign.toAIGAssignment
+    ⟧
+      =
+    ⟦aig, ⟨start, inv, hstart⟩, assign.toAIGAssignment⟧ := by
+  apply denote.eq_of_isPrefix (entry := ⟨aig, start, inv, hstart⟩)
+  apply IsPrefix.of
+  · intros
+    apply goCache_decl_eq
+  · intros
+    apply (goCache aig expr cache).result.property
+
+mutual
+
+
+theorem goCache_Inv_of_Inv (cache : Cache aig) (hinv : Cache.Inv assign aig cache) :
+    ∀ (expr : BVExpr w),
+        Cache.Inv assign (goCache aig expr cache).result.val.aig (goCache aig expr cache).cache := by
+  intro expr
+  generalize hres : goCache aig expr cache = res
+  unfold goCache at hres
+  split at hres
+  · rw [← hres]
+    exact hinv
+  · rw [← hres]
+    dsimp only
+    apply Cache.Inv_insert
+    · apply go_Inv_of_Inv
+      exact hinv
+    · intro idx hidx
+      rw [go_denote_eq]
+      exact hinv
+
+theorem go_Inv_of_Inv (cache : Cache aig) (hinv : Cache.Inv assign aig cache) :
+    ∀ (expr : BVExpr w),
+        Cache.Inv assign (go aig expr cache).result.val.aig (go aig expr cache).cache := sorry
+
+theorem goCache_denote_eq (aig : AIG BVBit) (expr : BVExpr w) (assign : Assignment)
+    (cache : Cache aig) (hinv : Cache.Inv assign aig cache) :
+    ∀ (idx : Nat) (hidx : idx < w),
+        ⟦(goCache aig expr cache).result.val.aig, (goCache aig expr cache).result.val.vec.get idx hidx, assign.toAIGAssignment⟧
+          =
+        (expr.eval assign).getLsbD idx := by
+  intro idx hidx
+  generalize hres : goCache aig expr cache = res
+  unfold goCache at hres
+  split at hres
+  · next heq =>
+    rw [← hres]
+    apply Cache.denote_eq_eval_of_get?_eq_some_of_Inv
+    · exact heq
+    · exact hinv
+  · rw [← hres]
+    rw [go_denote_eq]
+    exact hinv
+
+theorem go_denote_eq (aig : AIG BVBit) (expr : BVExpr w) (assign : Assignment)
+    (cache : Cache aig) (hinv : Cache.Inv assign aig cache) :
+    ∀ (idx : Nat) (hidx : idx < w),
+        ⟦(go aig expr cache).result.val.aig, (go aig expr cache).result.val.vec.get idx hidx, assign.toAIGAssignment⟧
+          =
+        (expr.eval assign).getLsbD idx := by
+  intro idx hidx
+  generalize hres : go aig expr cache = res
+  unfold go at hres
+  split at hres
+  · rw [← hres]
+    simp
+  · rw [← hres]
+    simp
+  · dsimp only at hres
+    split at hres
+    · rw [← hres]
+      simp
+      congr 1
+      · rw [goCache_denote_mem_prefix]
+        rw [goCache_denote_eq]
+        exact hinv
+      · rw [goCache_denote_eq]
+        apply goCache_Inv_of_Inv
+        exact hinv
+    · rw [← hres]
+      simp
+      congr 1
+      · rw [goCache_denote_mem_prefix]
+        rw [goCache_denote_eq]
+        exact hinv
+      · rw [goCache_denote_eq]
+        apply goCache_Inv_of_Inv
+        exact hinv
+    · rw [← hres]
+      simp
+      congr 1
+      · rw [goCache_denote_mem_prefix]
+        rw [goCache_denote_eq]
+        exact hinv
+      · rw [goCache_denote_eq]
+        apply goCache_Inv_of_Inv
+        exact hinv
+    · rw [← hres]
+      simp
+      rw [denote_blastAdd]
+      · intro idx hidx
+        rw [goCache_denote_mem_prefix]
+        simp
+        rw [goCache_denote_eq]
+        · exact hinv
+        · simp [Ref.hgate]
+      · intro idx hidx
+        rw [goCache_denote_eq]
+        apply goCache_Inv_of_Inv
+        exact hinv
+    · rw [← hres]
+      simp
+      rw [denote_blastMul]
+      · intro idx hidx
+        rw [goCache_denote_mem_prefix]
+        simp
+        rw [goCache_denote_eq]
+        · exact hinv
+        · simp [Ref.hgate]
+      · intro idx hidx
+        rw [goCache_denote_eq]
+        apply goCache_Inv_of_Inv
+        exact hinv
+    · rw [← hres]
+      simp
+      rw [denote_blastUdiv]
+      · intro idx hidx
+        rw [goCache_denote_mem_prefix]
+        simp
+        rw [goCache_denote_eq]
+        · exact hinv
+        · simp [Ref.hgate]
+      · intro idx hidx
+        rw [goCache_denote_eq]
+        apply goCache_Inv_of_Inv
+        exact hinv
+    · rw [← hres]
+      simp
+      rw [denote_blastUmod]
+      · intro idx hidx
+        rw [goCache_denote_mem_prefix]
+        simp
+        rw [goCache_denote_eq]
+        · exact hinv
+        · simp [Ref.hgate]
+      · intro idx hidx
+        rw [goCache_denote_eq]
+        apply goCache_Inv_of_Inv
+        exact hinv
+  · dsimp only at hres
+    split at hres
+    · rw [← hres]
+      simp [hidx]
+      rw [goCache_denote_eq]
+      · apply BitVec.getLsbD_eq_getElem
+      · exact hinv
+    · rw [← hres]
+      simp [hidx]
+      split
+      all_goals
+      · rw [goCache_denote_eq]
+        · apply BitVec.getLsbD_eq_getElem
+        · exact hinv
+    · rw [← hres]
+      simp [hidx]
+      split
+      all_goals
+      · rw [goCache_denote_eq]
+        · apply BitVec.getLsbD_eq_getElem
+        · exact hinv
+    · rw [← hres]
+      simp [hidx, BitVec.getElem_sshiftRight]
+      split
+      · rw [goCache_denote_eq]
+        · apply BitVec.getLsbD_eq_getElem
+        · exact hinv
+      · rw [goCache_denote_eq]
+        · simp [BitVec.msb_eq_getLsbD_last]
+        · exact hinv
+  · rw [← hres]
+    simp [BitVec.getLsbD_append, ]
+    split
+    · rw [goCache_denote_eq]
+      · sorry
+      · apply goCache_Inv_of_Inv
+        exact hinv
+    · sorry
+  · sorry
+  · rw [← hres]
+    simp [hidx]
+    split
+    · rw [goCache_denote_eq]
+      exact hinv
+    · symm
+      apply BitVec.getLsbD_ge
+      omega
+  · sorry
+  · sorry
+  · sorry
+
+end
+
+
+end bitblast
 
 @[simp]
 theorem denote_bitblast (aig : AIG BVBit) (expr : BVExpr w) (assign : Assignment) :
@@ -213,10 +365,11 @@ theorem denote_bitblast (aig : AIG BVBit) (expr : BVExpr w) (assign : Assignment
         ⟦(bitblast aig expr).aig, (bitblast aig expr).vec.get idx hidx, assign.toAIGAssignment⟧
           =
         (expr.eval assign).getLsbD idx
-    := mySorry
-  --intros
-  --rw [← bitblast.go_val_eq_bitblast]
-  --rw [bitblast.go_denote_eq]
+    := by
+  intros
+  rw [← bitblast.goCache_val_eq_bitblast]
+  rw [bitblast.goCache_denote_eq]
+  apply Cache.Inv_empty
 
 end BVExpr
 
